Defined ghost resources for reconf; Qed ghost_commit; may need to
rework the proof as additional "side-conditions" are added to make the
become_leader lemma work.

src/program_proof/reconf/ghost_proof.v
@@ -1,74 +1,11 @@
 From Perennial.program_proof Require Import grove_prelude.
 From iris.bi.lib Require Import fractional.
 From iris.algebra Require Import gmap cmra dfrac_agree.
-From iris.algebra Require Import sts.
+From iris.algebra Require Import mono_list.
 From iris.base_logic Require Import mono_nat.
 From iris.proofmode Require Import proofmode.
 
-Section poset_cmra.
-(*
-  Given poset (⪯, S), we want a cmra such that
-  x ~~> y iff x ⪯ y.
-
-  Carrier is (option S).
-  x ⋅ y = None, if x ⪯̸ y ∧ y ⪯̸ x
-  x ⋅ y = x if y ⪯ x
- *)
-
-Context `{T:Type}.
-Context `{R:relation T}.
-Context `{!PartialOrder R}.
-Context `{H: ∀ (x y:T), Decision (R x y)}.
-
-Definition poset_cmra_car := leibnizO (option T).
-
-Local Instance poset_op_instance : Op poset_cmra_car :=
-  λ ox oy,
-    x ← ox ;
-    y ← oy ;
-    if (decide (R x y)) then
-      Some y
-    else
-    if (decide (R y x)) then
-      Some x
-    else
-      None
-.
-
-Local Instance poset_pcore_instance : PCore poset_cmra_car := λ x, Some x.
-Local Instance poset_valid_instance : Valid poset_cmra_car := λ ox, is_Some ox.
-Local Instance poset_validN_instance : ValidN poset_cmra_car := λ _ ox, is_Some ox.
-
-Lemma poset_ra_mixin : RAMixin poset_cmra_car.
-Proof.
-  apply ra_total_mixin; try naive_solver.
-  - intros. intros z w. intros. destruct z, w; naive_solver.
-  - intros z w H1. eauto.
-  - intros z w. intros.
-    unfold impl.
-    intros.
-    unfold validN.
-    unfold poset_validN_instance.
-    naive_solver.
-  - intros x y z.
-    admit.
-Admitted.
-
-Canonical Structure posetR := Cmra (poset_cmra_car) (discrete_cmra_mixin _ poset_ra_mixin).
-
-End poset_cmra.
-
 Section ghost_proof.
-
-Record reconf_names :=
-{
-  acc_gn:gname
-}.
-
-Implicit Type γ:reconf_names.
-Implicit Type srv:u64.
-
-Context `{!heapGS Σ}.
 
 (* A configuration is known by its write quorums *)
 Record ConfigC :=
@@ -76,80 +13,90 @@ Record ConfigC :=
   is_quorum : (gset chan) → Prop
 }.
 
-Definition conf_eq (config1 config2:ConfigC) :=
-  ∀ W, config1.(is_quorum) W ↔ config2.(is_quorum) W.
-
-Record MonotonicValueC :=
+Record LogEntry :=
 {
-  version:u64 ;
   config:ConfigC ;
   val:list u8 ;
 }.
 
-Definition mval_le mval mval' := int.nat mval.(version) ≤ int.nat mval'.(version)
-                                    ∧ (mval.(version) = mval'.(version) → mval = mval')
-.
+Class reconfG Σ :=
+{
+  acc_inG:> inG Σ (gmapR (u64 * u64) (mono_listR (leibnizO LogEntry)));
+  commit_inG:> inG Σ (mono_listR (leibnizO LogEntry));
+  proposal_inG:> inG Σ (gmapR u64 (mono_listR (leibnizO LogEntry)));
+}.
 
-Definition mval_lt mval mval' := int.nat mval.(version) < int.nat mval'.(version).
+Record reconf_names :=
+{
+  acc_gn:gname ;
+  commit_gn:gname ;
+  prop_gn:gname ;
+}.
 
-Implicit Type mval:MonotonicValueC.
+Implicit Type γ:reconf_names.
+Implicit Type srv:u64.
+
+Context `{!heapGS Σ}.
+Context `{!reconfG Σ}.
+
+Definition conf_eq (config1 config2:ConfigC) :=
+  ∀ W, config1.(is_quorum) W ↔ config2.(is_quorum) W.
+
+Implicit Type mval : (list (leibnizO LogEntry)).
+
+Definition mval_le mval mval' := prefix mval mval'.
+
+Definition mval_lt mval mval' := prefix mval mval' ∧ mval ≠ mval'.
+
 Implicit Type term:u64.
 
 (* This is just ownership of raw ghost resources. *)
 
-Definition accepted γ srv term mval : iProp Σ.
+Definition def_config : ConfigC.
 Admitted.
 
-Definition accepted_ro γ srv term mval : iProp Σ.
-Admitted.
+Definition get_config mval : ConfigC :=
+  match (last mval) with
+  | Some e => e.(config)
+  | _ => def_config
+end
+.
 
-Definition accepted_ro_none γ srv term : iProp Σ.
-Admitted.
+Definition accepted γ srv term mval : iProp Σ :=
+  own γ.(acc_gn) {[ (term,srv) := ●ML mval ]}.
 
-Definition accepted_lb γ srv term mval : iProp Σ.
-Admitted.
+Definition accepted_ro γ srv term mval : iProp Σ :=
+  own γ.(acc_gn) {[ (term,srv) := ●ML□ mval ]}.
 
-Definition commit γ mval : iProp Σ.
-Admitted.
+Definition accepted_ro_none γ srv term : iProp Σ :=
+  own γ.(acc_gn) {[ (term,srv) := ●ML□ [] ]}. (* XXX: not sure if empty list is good enough here*)
 
-Definition commit_lb γ mval : iProp Σ.
-Admitted.
+Definition accepted_lb γ srv term mval : iProp Σ :=
+  own γ.(acc_gn) {[ (term,srv) := ◯ML mval ]}.
 
-Definition proposed γ term mval : iProp Σ.
-Admitted.
+Definition commit γ mval : iProp Σ :=
+  own γ.(commit_gn) (●ML mval).
 
-Definition proposed_lb γ term mval : iProp Σ.
-Admitted.
+Definition commit_lb γ mval : iProp Σ :=
+  own γ.(commit_gn) (◯ML mval).
 
-Instance commit_timeless γ mval : Timeless (commit γ mval).
-Admitted.
+Definition proposed γ term mval : iProp Σ :=
+  own γ.(acc_gn) {[ term := ●ML mval ]}.
 
-Instance accepted_lb_timeless γ srv term mval : Timeless (accepted_lb γ srv term mval).
-Admitted.
+Definition proposed_lb γ term mval : iProp Σ :=
+  own γ.(acc_gn) {[ term := ◯ML mval ]}.
 
-Instance commit_lb_pers γ mval : Persistent (commit_lb γ mval).
-Admitted.
-
-Instance proposed_lb_pers γ term mval : Persistent (proposed_lb γ term mval).
-Admitted.
-
-
-Instance accepted_ro_pers γ srv term mval : Persistent (accepted_ro γ srv term mval).
-Admitted.
-
-Instance accepted_lb_pers γ srv term mval : Persistent (accepted_lb γ srv term mval).
-Admitted.
 
 (* This is more complicated stuff, beyond raw ghost resource ownership. *)
 
 Definition committed_at_term γ term mval: iProp Σ :=
-  ∃ W, ⌜mval.(config).(is_quorum) W⌝ ∗
+  ∃ W, ⌜(get_config mval).(is_quorum) W⌝ ∗
   ([∗ set] srv ∈ W, accepted_lb γ srv term mval)
 .
 
 Definition old_conf_max γ term mval : iProp Σ :=
-  ∀ term', ⌜int.nat term' < int.nat term⌝ →
-  (∀ mval', (committed_at_term γ term' mval') →
+  □(∀ term' mval', ⌜int.nat term' < int.nat term⌝ →
+  (committed_at_term γ term' mval') -∗
             ⌜mval_le mval' mval⌝
   )
 .
@@ -160,7 +107,11 @@ Definition sys_inv γ : iProp Σ :=
   inv sysN (
         ∃ term mval,
           commit γ mval ∗
-          (committed_at_term γ term mval)
+          (committed_at_term γ term mval) ∗
+          proposed_lb γ term mval ∗
+          old_conf_max γ term mval (* XXX: could make a accepted_lb_fancy, and put this
+                              in there, and add requirement that quorum is
+                              non-empty. *)
   ).
 
 Definition overlapping_quorums (config1 config2:ConfigC) :=
@@ -172,9 +123,9 @@ Definition no_concurrent_reconfigs_and_overlapping_quorums γ term mval : iProp 
       ∀ mval'', ⌜mval_lt mval'' mval⌝ →
                 ⌜mval_le mval' mval''⌝ →
                 proposed_lb γ term mval'' →
-                ⌜conf_eq mval'.(config) mval''.(config)⌝
+                ⌜conf_eq (get_config mval') (get_config mval'')⌝
     ) ∗
-    ⌜overlapping_quorums mval.(config) mval'.(config)⌝
+    ⌜overlapping_quorums (get_config mval) (get_config mval')⌝
 .
 
 Definition proposed_lb_fancy γ term mval : iProp Σ :=
@@ -182,23 +133,98 @@ Definition proposed_lb_fancy γ term mval : iProp Σ :=
   no_concurrent_reconfigs_and_overlapping_quorums γ term mval
 .
 
+Lemma mono_list_included': ∀ (A : ofe) (dq : dfrac) (l l': list A),
+    l `prefix_of` l' →
+    ◯ML l ≼ ●ML{dq} l'.
+Proof.
+  intros.
+  assert (◯ML l' ≼ ●ML{dq} l').
+  { apply mono_list_included. }
+  assert (◯ML l ≼ ◯ML l').
+  { apply mono_list_lb_mono. done. }
+  apply (transitivity H1 H0).
+Qed.
+
 Lemma ghost_commit γ term mval :
   sys_inv γ -∗
-  committed_at_term γ term mval ={↑sysN}=∗
+  committed_at_term γ term mval -∗
+  proposed_lb γ term mval -∗
+  old_conf_max γ term mval (* XXX: could make a accepted_lb_fancy, and put this
+                              in there, and add requirement that quorum is
+                              non-empty. *)
+  ={↑sysN}=∗
   commit_lb γ mval
 .
 Proof.
-  iIntros "#Hinv #Hcommit".
-  iDestruct "Hcommit" as (W) "[%Hquorum Hacc]".
+  iIntros "#Hinv #HcommitAt #Hproposed #Hold".
   iInv "Hinv" as ">Hi" "Hclose".
-  iDestruct "Hi" as (commitTerm commitVal) "[Hcommit HcommitAcc]".
-  iDestruct "HcommitAcc" as (Wcom) "[%Hcom_quorum HcommitAcc]".
-Admitted.
+  iDestruct "Hi" as (commitTerm commitVal) "(Hcommit & #HcommitAcc & #HproposedCommit & #HoldCommit)".
+  iAssert (⌜mval_le mval commitVal ∨ mval_le commitVal mval⌝)%I as "%Hcomparable".
+  {
+    destruct (decide (int.nat term < int.nat commitTerm)).
+    { (* case: term < commitTerm *)
+      iDestruct ("HoldCommit" with "[] HcommitAt") as "%HvalLe".
+      { done. }
+      eauto.
+    }
+    destruct (decide (int.nat term = int.nat commitTerm)).
+    { (* case: term == commitTerm *)
+      replace (commitTerm) with (term) by word.
+      (* TODO: put together the proposed_lb's to know that one of them is bigger
+       than the other. *)
+      iDestruct (own_valid_2 with "Hproposed HproposedCommit") as %Hvalid.
+      rewrite singleton_op in Hvalid.
+      apply singleton_valid in Hvalid.
+      apply mono_list_lb_op_valid_1_L in Hvalid.
+      done.
+    }
+    (* case: term > commitTerm *)
+    assert (int.nat term > int.nat commitTerm) by word.
+    iDestruct ("Hold" with "[] HcommitAcc") as "%HvalLe".
+    { done. }
+    eauto.
+  }
+
+  destruct Hcomparable.
+  { (* committed value is bigger than mval *)
+    iDestruct (own_mono _ _ (◯ML mval) with "Hcommit") as "#HH".
+    {
+      by apply mono_list_included'.
+    }
+    iFrame "#".
+    iMod ("Hclose" with "[Hcommit]").
+    {
+      iNext.
+      iExists _, _; iFrame.
+      iFrame "#".
+    }
+    done.
+  }
+  { (* mval is bigger than committed value; in this case, we commit something new *)
+    iMod (own_update with "Hcommit") as "Hcommit".
+    {
+      apply mono_list_update.
+      exact H.
+    }
+    iDestruct (own_mono _ _ (◯ML mval) with "Hcommit") as "#HH".
+    {
+      apply mono_list_included.
+    }
+    iFrame "#".
+    iMod ("Hclose" with "[Hcommit]").
+    {
+      iNext.
+      iExists _, _; iFrame.
+      iFrame "#".
+    }
+    done.
+  }
+Qed.
 
 Lemma become_leader γ term highestVal :
   ∀ highestTerm W,
     int.nat highestTerm < int.nat term →
-    highestVal.(config).(is_quorum) W →
+    (get_config highestVal).(is_quorum) W →
     sys_inv γ -∗
     proposed_lb_fancy γ highestTerm highestVal -∗
     □(
